theories/L/Complexity/Problems/GenNPHalt.v
@@ -1,15 +1,20 @@
 From Undecidability.L Require Import L.
 From Undecidability.L.Datatypes Require Import LProd LTerm LBool.
-From Undecidability.L.Complexity Require Import NP Synthetic Monotonic GenNP.
+From Undecidability.L.Complexity Require Import NP Synthetic Monotonic.
 From Undecidability.L.Functions Require Import Size.
 
-Definition GenNPHalt : term*nat*nat -> Prop :=
+Definition GenNPHalt' : term*nat*nat -> Prop :=
   fun '(s, maxSize, steps (*in unary*)) =>
-    closed s /\
     exists (c:term), size (enc c) <= maxSize
                 /\ exists t, s (enc c) ⇓(<=steps) t.
 
-Lemma NPhard_GenNP : NPhard (unrestrictedP GenNPHalt).
+Definition HaltsOrDiverges : term*nat*nat -> Prop :=
+  fun '(s, maxSize, steps (*in unary*)) =>
+    closed s /\ forall (c:term), size (enc c) <= maxSize -> ~(exists t, s (enc c) ⇓ t) \/ exists t, s (enc c) ⇓(<=steps) t.
+
+Definition GenNPHalt := restrictBy HaltsOrDiverges GenNPHalt'.
+
+Lemma NPhard_GenNP : NPhard GenNPHalt.
 Proof.
   intros X reg__X ? Q [(*? ?*) R R__dec (f__Rbal&polyf__Rbal&bounds_f__Rbal&mono_f__Rbal) R__spec].
   destruct R__dec as (t__R&[d__R [comp_d__R] spec_d__R]&poly_t__R&mono_t__R).
@@ -18,8 +23,9 @@ Proof.
   {intros. subst f. extract. solverec. }
   specialize inOPoly_computable with (1:=polyf__Rbal) as (f__Rbal'&tf__Rbal'&[]&polyf__Rbal'&leq_f__Rbal'&?&?&?).
   specialize inOPoly_computable with (1:=poly_t__R) as (t__R'&tt__R'&[]&poly_t__R'&leq_t__R'&?&?&?).
-  exists (fun x => (lam (trueOrDiverge (extT f (enc x) 0)),f__Rbal' (size (enc x)),t__R' (size (enc x) + f__Rbal' (size (enc x))+4)+9));cbn [fst snd GenNP]. 3:easy. 
-  -evar (f':nat -> nat). [f']:refine (fun x => _).
+  pose (g:= fun x => (lam (trueOrDiverge (extT f (enc x) 0)),f__Rbal' (size (enc x)),t__R' (size (enc x) + f__Rbal' (size (enc x))+4)+9)).
+  apply reducesPolyMO_intro with (f:= g);cbn [fst snd]. 
+  -unfold g. evar (f':nat -> nat). [f']:refine (fun x => _).
    eexists (fun x => f' x). 
    +split. extract.
     recRel_prettify2. cbn [size].  generalize (size (enc x)). intro. unfold f'. reflexivity. 
@@ -32,32 +38,43 @@ Proof.
      generalize (size (enc x)). intros. reflexivity.
     *smpl_inO. all:eapply inOPoly_comp. all:smpl_inO.
     *smpl_inO.
-  -intros x ?.
-   rewrite R__spec. 2:easy. split.
-   +intros (c&H'). specialize (spec_d__R (x,c)). apply ssreflect.iffLR with (2:=H') in spec_d__R. 2:easy. 
-    unfold GenNPHalt.
-    split. now Lproc.
-    exists c. repeat split. 
-    *rewrite bounds_f__Rbal. 2:eassumption. easy.
-    *exists I. split. 2:Lproc. 
-     eapply le_redLe_proper. 2,3:reflexivity.
-     2:{eapply redLe_trans_eq.
-        2:now Lsimpl.
-        2:{unfold f. rewrite spec_d__R. Lsimpl.
-        }
-     cbn [fst snd]. reflexivity. }
-     ring_simplify.
-     rewrite <- leq_t__R'. cbn.
-     rewrite size_prod. cbn [fst snd].
-     hnf in mono_t__R;rewrite mono_t__R. reflexivity.
-     rewrite bounds_f__Rbal. 2:eassumption.
-     rewrite leq_f__Rbal'. reflexivity.
-   +unfold GenNPHalt.
-    intros (?&c&size__c&?&R'%redLe_star_subrelation&?).    
-    exists c. specialize (spec_d__R (x,c)). cbn in spec_d__R. rewrite spec_d__R. 2:easy. 
-    eapply trueOrDiverge_eval with (t:=x0).
-    eapply equiv_eval_proper. 2:reflexivity. 2:apply eval_refl;Lproc.
-    rewrite <- R'. clear R'.
-    apply star_equiv.
-    Lbeta. eapply redLe_star_subrelation. Lsimpl.
+  -intros x ?. remember (g x) as x0 eqn:eqx0. destruct x0 as ((t0,maxSize0),steps0).
+   unfold g in eqx0. injection eqx0. intros Hx0 Hsize0 Hsteps0.  clear eqx0.
+   rewrite R__spec. 2:easy. cbn [GenNPHalt restrictBy fst snd].
+   unfold HaltsOrDiverges,GenNPHalt'.
+   evar (c0 : nat).
+   assert (Ht0 : forall c, size (enc c) <= maxSize0 -> t0 (enc c) >(<= c0) trueOrDiverge (enc (f x c))).
+   {intros c Hc. subst t0. eapply le_redLe_proper. 2,3:reflexivity. 2:Lsimpl.
+    cbn [fst snd]. ring_simplify.
+    rewrite size_prod. cbn [fst snd].
+    hnf in mono_t__R;erewrite mono_t__R. rewrite leq_t__R'.
+    2:now rewrite Hc. 
+    unfold c0. reflexivity. }
+   unshelve eapply (_ : forall (A B : Prop), A -> (A -> B) -> A /\ B). tauto. 
+   +split. now subst t0;Lproc.
+    intros c H'. specialize (Ht0 c).
+    destruct (f x c) eqn:eqfxc.
+    *right. eexists. eapply le_evalLe_proper. 2,3:reflexivity. 2:now Lsimpl.
+     unfold c0. subst steps0. ring_simplify. 
+     subst maxSize0. nia. 
+    *left. intros [? Rc].
+     apply Ht0 in H'. eapply redLe_star_subrelation in H'. rewrite H' in Rc.
+     eapply trueOrDiverge_eval in Rc. easy.    
+   +intros [_ Hc]. split.
+    *intros (c&H'). specialize (spec_d__R (x,c) H6). cbn [fst snd] in *.
+     exists c. split. 
+     --rewrite bounds_f__Rbal. 2:eassumption. subst;easy.
+     --exists I.
+       unshelve eassert (Hc'' := Ht0 _ _). 2:{rewrite bounds_f__Rbal. 2:easy. subst maxSize0. now apply leq_f__Rbal'. }
+       eapply le_evalLe_proper. 2,3:reflexivity.
+       2:{Lsimpl. unfold f. rewrite (proj1 spec_d__R). 2:easy. Lsimpl. }
+       subst steps0 c0. cbn beta. ring_simplify. subst maxSize0. nia.
+    *intros (c&size__c&?&R').    
+     exists c. specialize (spec_d__R (x,c)). cbn in spec_d__R. rewrite spec_d__R. 2:easy. 
+     eapply trueOrDiverge_eval with (t:=x0).
+     eapply equiv_eval_proper. 2:reflexivity.
+     {unfold f in Ht0. specialize (Ht0 _ size__c). apply redLe_star_subrelation in  Ht0.  rewrite <- Ht0.
+      symmetry. apply star_equiv_subrelation. eapply redLe_star_subrelation. apply R'.
+     }
+     apply eval_refl. now destruct R'.
 Qed.
